Experiment

src/defs.lean
@@ -11,6 +11,7 @@ inductive expr : Type
 | pi   : expr → expr → expr
 open expr
 
+/-- Debug output. -/
 def expr.show : expr → string
 | (sort s)   := "Sort " ++ to_string s
 | (var v)    := "#" ++ to_string v
@@ -25,12 +26,105 @@ def expr.show : expr → string
 instance : has_to_string expr := ⟨expr.show⟩
 instance : has_repr expr := ⟨expr.show⟩
 
+/-- Size measure for strong induction. -/
+def expr.size : expr → nat
+| (sort s)   := 1
+| (var v)    := 1
+| (app l r)  := nat.succ (expr.size l + expr.size r)
+| (lam t e)  := nat.succ (expr.size t + expr.size e)
+| (pi t₁ t₂) := nat.succ (expr.size t₁ + expr.size t₂)
+
+/-- Lift variables with level ≥ `n` by `m` levels. -/
+@[irreducible]
+def expr.shift : expr → nat → nat → expr
+| (sort s)   n m := sort s
+| (var v)    n m := if n <= v then var (v + m) else var v
+| (app l r)  n m := app (expr.shift l n m) (expr.shift r n m)
+| (lam t e)  n m := lam (expr.shift t n m) (expr.shift e (nat.succ n) m)
+| (pi t₁ t₂) n m := pi (expr.shift t₁ n m) (expr.shift t₂ (nat.succ n) m)
+
+/-- Replace all variables at level = `n` by an expression `e'`
+    (when deleting the outermost layer of binder). -/
+@[irreducible]
+def expr.subst : expr → nat → expr → expr
+| (sort s)   n e' := sort s
+| (var v)    n e' := if n < v then var (nat.pred v) else if n = v then expr.shift e' 0 n else var v
+| (app l r)  n e' := app (expr.subst l n e') (expr.subst r n e')
+| (lam t e)  n e' := lam (expr.subst t n e') (expr.subst e (nat.succ n) e')
+| (pi t₁ t₂) n e' := pi (expr.subst t₁ n e') (expr.subst t₂ (nat.succ n) e')
+
+/-- Small-step reduction rules. -/
+inductive small : expr → expr → Prop
+| s_beta      {t e r}     : small (app (lam t e) r) (expr.subst e 0 r)
+| s_app_left  {l l' r}    : small l l' →   small (app l r) (app l' r)
+| s_app_right {l r r'}    : small r r' →   small (app l r) (app l r')
+| s_lam_left  {t t' e}    : small t t' →   small (lam t e) (lam t' e)
+| s_lam_right {t e e'}    : small e e' →   small (lam t e) (lam t e')
+| s_pi_left   {t₁ t₁' t₂} : small t₁ t₁' → small (pi t₁ t₂) (pi t₁' t₂)
+| s_pi_right  {t₁ t₂ t₂'} : small t₂ t₂' → small (pi t₁ t₂) (pi t₁ t₂')
+open small
+
+/-- Transitive closure of small-step reduction rules. -/
+inductive small_star : expr → expr → Prop
+| ss_refl {e}        :                                  small_star e e
+| ss_step {e₁ e₂ e₃} : small_star e₁ e₂ → small e₂ e₃ → small_star e₁ e₃
+open small_star
+
+/-- Symmetric transitive closure of small-step reduction rules. -/
+inductive small_eq : expr → expr → Prop
+| se_refl  {e}        :                                   small_eq e e
+| se_step  {e₁ e₂}    : small e₁ e₂ →                     small_eq e₁ e₂
+| se_symm  {e₁ e₂}    : small_eq e₁ e₂ →                  small_eq e₂ e₁
+| se_trans {e₁ e₂ e₃} : small_eq e₁ e₂ → small_eq e₂ e₃ → small_eq e₁ e₃
+open small_eq
+
 /-- Contexts (precontexts) -/
 def ctx : Type := list expr
 
 instance : has_to_string ctx := ⟨list.to_string⟩
 instance : has_repr ctx := ⟨list.to_string⟩
 instance : has_append ctx := ⟨list.append⟩
+
+/-- Lean 3 does not primitively support mutually inductive types. -/
+@[derive decidable_eq]
+inductive judgment_index
+| well_ctx : ctx →               judgment_index
+| has_type : ctx → expr → expr → judgment_index
+open judgment_index
+
+/-- Typing rules. -/
+inductive judgment : judgment_index → Prop
+| c_nil :
+  judgment (well_ctx [])
+| c_cons {Γ t s} :
+  judgment (well_ctx Γ) →
+  judgment (has_type Γ t (sort s)) →
+  judgment (well_ctx (t :: Γ))
+| t_conv {Γ e t t' s} :
+  small_eq t t' →
+  judgment (has_type Γ t' (sort s)) →
+  judgment (has_type Γ e t) →
+  judgment (has_type Γ e t')
+| t_sort {Γ n} :
+  judgment (well_ctx Γ) →
+  judgment (has_type Γ (sort n) (sort (nat.succ n)))
+| t_var {Γ n t} :
+  judgment (well_ctx Γ) →
+  list.nth Γ n = option.some t →
+  judgment (has_type Γ (var n) (expr.shift t 0 (nat.succ n)))
+| t_app {Γ l r t₁ t₂} :
+  judgment (has_type Γ l (pi t₁ t₂)) →
+  judgment (has_type Γ r t₁) →
+  judgment (has_type Γ (app l r) (expr.subst t₂ 0 r))
+| t_lam {Γ t₁ t₂ s e} :
+  judgment (has_type Γ (pi t₁ t₂) (sort s)) →
+  judgment (has_type (t₁ :: Γ) e t₂) →
+  judgment (has_type Γ (lam t₁ e) (pi t₁ t₂))
+| t_pi {Γ t₁ s₁ t₂ s₂} :
+  judgment (has_type Γ t₁ (sort s₁)) →
+  judgment (has_type (t₁ :: Γ) t₂ (sort s₂)) →
+  judgment (has_type Γ (pi t₁ t₂) (sort (max s₁ s₂)))
+open judgment
 
 end
 end coc
